Perform a massive renaming [access_location] -> [location]

vale/code/lib/transformers/Vale.Transformers.AccessLocations.fsti
@@ -11,82 +11,82 @@ open Vale.Transformers.PossiblyMonad
 
 module L = FStar.List.Tot
 
-(** An [access_location] is a portion of the [machine_state] that may
-    be independently modified and/or accessed. *)
-val access_location : eqtype
+(** An [location] is a portion of the [machine_state] that may be
+    independently modified and/or accessed. *)
+val location : eqtype
 
 unfold
-type access_locations = list access_location
+type locations = list location
 
-(** An [rw_set] is the pair of [access_locations] that are
-    respectively read and written by an operation. *)
-type rw_set = access_locations & access_locations
+(** An [rw_set] is the pair of [locations] that are respectively read
+    and written by an operation. *)
+type rw_set = locations & locations
 
 (** [rw_set_of_ins i] returns the read/write sets for the execution of
     an instruction. *)
 val rw_set_of_ins : i:ins -> rw_set
 
-(** [disjoint_access_location a1 a2] is true whenever [a1] and [a2]
+(** [disjoint_location a1 a2] is true whenever locations [a1] and [a2]
     are disjoint. When not disjoint, it gives a reason for why not. *)
-val disjoint_access_location : access_location -> access_location -> pbool
+val disjoint_location : location -> location -> pbool
 
 (** Disjointness is the same as syntactic equality on the locations. *)
-val lemma_disjoint_access_location :
-  a1:access_location -> a2:access_location ->
+val lemma_disjoint_location :
+  a1:location -> a2:location ->
   Lemma
-    (ensures (!!(disjoint_access_location a1 a2) = (a1 <> a2)))
+    (ensures (!!(disjoint_location a1 a2) = (a1 <> a2)))
 
-(** Disjointness of an [access_location] from [access_locations] *)
-let disjoint_access_location_from_locations (a:access_location) (l:access_locations) : pbool =
+(** Disjointness of a [location] from [locations] *)
+let disjoint_location_from_locations (a:location) (l:locations) : pbool =
   for_all (fun b ->
-      disjoint_access_location a b
+      disjoint_location a b
     ) l
 
-(** Disjointness of [access_locations] *)
-let disjoint_access_locations (l1 l2:access_locations) : pbool =
+(** Disjointness of [locations] *)
+let disjoint_locations (l1 l2:locations) : pbool =
   for_all (fun x ->
-      disjoint_access_location_from_locations x l2
+      disjoint_location_from_locations x l2
   ) l1
 
-(** [disjoint_access_locations] is symmetric *)
-let rec lemma_disjoint_access_locations_symmetric l1 l2 :
+(** [disjoint_locations] is symmetric *)
+let rec lemma_disjoint_locations_symmetric l1 l2 :
   Lemma
     (ensures (
-        (!!(disjoint_access_locations l1 l2) = !!(disjoint_access_locations l2 l1))))
+        (!!(disjoint_locations l1 l2) = !!(disjoint_locations l2 l1))))
     (decreases %[L.length l1 + L.length l2]) =
   match l1, l2 with
   | [], [] -> ()
   | [], x :: xs | x :: xs, [] ->
-    lemma_disjoint_access_locations_symmetric xs []
+    lemma_disjoint_locations_symmetric xs []
   | x :: xs, y :: ys ->
-    lemma_disjoint_access_location x y;
-    lemma_disjoint_access_location y x;
-    lemma_disjoint_access_locations_symmetric l1 ys;
-    lemma_disjoint_access_locations_symmetric xs l2;
-    lemma_disjoint_access_locations_symmetric xs ys
+    lemma_disjoint_location x y;
+    lemma_disjoint_location y x;
+    lemma_disjoint_locations_symmetric l1 ys;
+    lemma_disjoint_locations_symmetric xs l2;
+    lemma_disjoint_locations_symmetric xs ys
 
-(** [access_location_val_t a] is the type of the value represented by the location [a]. *)
-val access_location_val_t : access_location -> Type0
+(** [location_val_t a] is the type of the value represented by the location [a]. *)
+val location_val_t : location -> Type0
 
-(** [eval_access_location a s] gives the value at location [a] in state [s]. *)
-val eval_access_location :
-  a:access_location ->
+(** [eval_location a s] gives the value at location [a] in state [s]. *)
+val eval_location :
+  a:location ->
   machine_state ->
-  access_location_val_t a
+  location_val_t a
 
-(** [update_access_location a v s0] gives a new state with [a] updated to [v]. *)
-val update_access_location :
-  a:access_location ->
-  v:access_location_val_t a ->
+(** [update_location a v s0] gives a new state with location [a] updated to [v]. *)
+val update_location :
+  a:location ->
+  v:location_val_t a ->
   machine_state ->
-  s:machine_state{eval_access_location a s == v}
+  s:machine_state{eval_location a s == v}
 
-(** Updating one access location does not affect other access locations *)
-val lemma_access_locations_truly_disjoint :
-  a:access_location ->
-  a_change:access_location ->
-  v:access_location_val_t a_change ->
+(** Updating one location does not affect a different location. *)
+val lemma_locations_truly_disjoint :
+  a:location ->
+  a_change:location ->
+  v:location_val_t a_change ->
   s:machine_state ->
   Lemma
     (requires (a <> a_change))
-    (ensures (eval_access_location a s == eval_access_location a (update_access_location a_change v s)))
+    (ensures (eval_location a s == eval_location a (update_location a_change v s)))
